work on IL4 translation correctness
bite the bullet and use the good_v_i2 predicate and prove evaluate_i3
preserves it...

attempting to prove things about pat_to_i4 and it's surprisingly subtle
and long, but basically going through.

finished skeleton of exp_to_i4_correct, with cheats mostly for pattern
matching.

compiler/proofs/toIntLang4ProofScript.sml
@@ -65,16 +65,26 @@ val v_to_i4_def = save_thm("v_to_i4_def",
   v_to_i4_def |> SIMP_RULE (srw_ss()++ETA_ss) [MAP_MAP_o])
 val _ = export_rewrites["v_to_i4_def"]
 
-val good_v_i2_def = Define`
+val good_v_i2_def = tDefine"good_v_i2"`
   (good_v_i2 (Litv_i2 _) ⇔ T) ∧
-  (good_v_i2 (Conv_i2 _ _) ⇔ T) ∧
-  (good_v_i2 (Closure_i2 _ _ _) ⇔ T) ∧
-  (good_v_i2 (Recclosure_i2 _ funs f) ⇔
+  (good_v_i2 (Conv_i2 _ vs) ⇔ good_vs_i2 vs) ∧
+  (good_v_i2 (Closure_i2 env _ _) ⇔ good_vs_i2 (MAP SND env)) ∧
+  (good_v_i2 (Recclosure_i2 env funs f) ⇔
+   good_vs_i2 (MAP SND env) ∧
    ALL_DISTINCT (MAP FST funs) ∧ MEM f (MAP FST funs)) ∧
   (good_v_i2 (Loc_i2 _) ⇔ T) ∧
   (good_vs_i2 [] ⇔ T) ∧
   (good_vs_i2 (v::vs) ⇔ good_v_i2 v ∧ good_vs_i2 vs)`
+(WF_REL_TAC`inv_image $< (\x. case x of INL v => v_i2_size v
+                                      | INR vs => v_i23_size vs)` >>
+ simp[] >> conj_tac >> rpt gen_tac >> Induct_on`env` >> simp[v_i2_size_def] >>
+ Cases >> simp[v_i2_size_def] >> rw[] >> res_tac >> simp[])
 val _ = export_rewrites["good_v_i2_def"]
+
+val good_vs_i2_EVERY = store_thm("good_vs_i2_EVERY",
+  ``∀vs. good_vs_i2 vs ⇔ EVERY good_v_i2 vs``,
+  Induct >> simp[])
+val _ = export_rewrites["good_vs_i2_EVERY"]
 
 (* TODO: move *)
 
@@ -127,7 +137,7 @@ val ALOOKUP_find_index_SOME = prove(
     ∃i. (find_index k (MAP FST env) 0 = SOME i) ∧
         i < LENGTH env ∧ (v = SND (EL i env))``,
   rw[] >> imp_res_tac ALOOKUP_find_index_SOME >>
-  imp_res_tac find_index_LESS_LENGTH >> fs[[L_MAP])
+  imp_res_tac find_index_LESS_LENGTH >> fs[EL_MAP])
 val ALOOKUP_find_index_NONE = prove(
   ``(ALOOKUP env k = NONE) ⇒ (find_index k (MAP FST env) m = NONE)``,
   rw[ALOOKUP_FAILS] >> rw[GSYM find_index_NOT_MEM,MEM_MAP,EXISTS_PROD])
@@ -207,35 +217,577 @@ val do_app_i4_correct = prove(
   asm_simp_tac(std_ss)[EL_MAP] >>
   simp[])
 
-(*
-val IS_SOME_exists = prove(
-  ``IS_SOME X ⇔ ∃x. X = SOME x``,
-  Cases_on`X`>>simp[])
+val good_env_s_i2_def = Define`
+  good_env_s_i2 env (s:v_i2 count_store_genv) ⇔
+    EVERY good_v_i2 (MAP SND env) ∧
+    EVERY good_v_i2 (SND (FST s)) ∧
+    EVERY (OPTION_EVERY good_v_i2) (SND s)`
 
-val do_app_i4_SOME = prove(
-  ``∀op v1 v2 env s env' s' exp'.
-     (do_app_i2 env s op v1 v2 = SOME (env',s',exp')) ⇒
-     (do_app_i4 (MAP (v_to_i4 o SND) env) (MAP v_to_i4 s) op (v_to_i4 v1) (v_to_i4 v2) =
-       SOME (MAP (v_to_i4 o SND) env', MAP v_to_i4 s', exp_to_i4 (MAP (SOME o FST) env') exp'))``,
+val do_uapp_i3_preserves_good = prove(
+  ``∀env s uop v s' v'. good_env_s_i2 env s ∧ good_v_i2 v ∧
+    (do_uapp_i3 (SND(FST s),SND s) uop v = SOME (s',v')) ⇒
+    good_env_s_i2 env ((FST(FST s),(FST s')),SND s') ∧
+    good_v_i2 v'``,
+  rpt gen_tac >> Cases_on`uop`>>EVAL_TAC>>
+  TRY(BasicProvers.CASE_TAC) >>
+  rw[] >>
+  fs[EVERY_MEM,EVERY_MAP] >>
+  TRY (fs[MEM_EL,PULL_EXISTS]>>NO_TAC) >>
+  rw[] >> imp_res_tac MEM_LUPDATE_E >> rw[])
+
+val do_app_i2_preserves_good = prove(
+  ``∀env s op v1 v2 env' s' exp'.
+     (do_app_i2 env s op v1 v2 = SOME (env', s', exp')) ∧
+     EVERY good_v_i2 (MAP SND env) ∧
+     EVERY good_v_i2 s ∧
+     good_v_i2 v1 ∧ good_v_i2 v2
+     ⇒
+     EVERY good_v_i2 (MAP SND env') ∧
+     EVERY good_v_i2 s'``,
   Cases_on`op`>>TRY(Cases_on`o':opn`)>>Cases_on`v1`>>TRY(Cases_on`l:lit`)>>Cases_on`v2`>>TRY(Cases_on`l:lit`)>>
-  simp[do_app_i2_def,do_app_i4_def,exn_env_i4_def,exn_env_i2_def
-      ,libTheory.emp_def,libTheory.bind_def,do_eq_i4_correct,do_eq_i4_def]>>rw[]>>
-  fs[find_recfun_ALOOKUP,funs_to_i4_MAP] >- (
-    BasicProvers.CASE_TAC >> simp[] >> fs[] >> rw[]) >>
-  pop_assum mp_tac >> BasicProvers.CASE_TAC >>
-  fs[optionTheory.option_case_compute,IS_SOME_exists] >> rfs[pair_CASE_def] >>
-  simp[the_less_rwt] >>
-  imp_res_tac ALOOKUP_find_index_SOME >>
-  rw[build_rec_env_i4_def,build_rec_env_i2_MAP] >>
-  simp[EL_MAP,MAP_MAP_o,combinTheory.o_DEF] >>
-  rw[LIST_EQ_REWRITE] >>
-  simp[EL_MAP,UNCURRY,funs_to_i4_MAP,MAP_MAP_o]
+  simp[do_app_i2_def,exn_env_i2_def,libTheory.emp_def,libTheory.bind_def,do_eq_i2_def]>>rw[]>>rw[]>>
+  last_x_assum mp_tac >> BasicProvers.CASE_TAC >> rw[] >> rw[] >>
+  fs[pair_CASE_def,semanticPrimitivesTheory.store_assign_def] >> rw[build_rec_env_i2_MAP] >>
+  fs[EVERY_MAP,EVERY_MEM,UNCURRY,MEM_MAP] >>
+  rw[] >> imp_res_tac MEM_LUPDATE_E >> rw[] >>
+  rw[EVERY_MAP,EVERY_MEM] >> metis_tac[MEM_MAP])
+
+val evaluate_i3_preserves_good = store_thm("evaluate_i3_preserves_good",
+  ``(∀ck env s exp res. evaluate_i3 ck env s exp res ⇒
+      good_env_s_i2 env s ⇒
+      good_env_s_i2 env (FST res) ∧
+      every_result good_v_i2 good_v_i2 (SND res)) ∧
+    (∀ck env s exps ress. evaluate_list_i3 ck env s exps ress ⇒
+      good_env_s_i2 env s ⇒
+      good_env_s_i2 env (FST ress) ∧
+      every_result good_vs_i2 good_v_i2 (SND ress)) ∧
+    (∀ck env s v pes ev res. evaluate_match_i3 ck env s v pes ev res ⇒
+      good_env_s_i2 env s ∧ good_v_i2 v ∧ good_v_i2 ev ⇒
+      good_env_s_i2 env (FST res) ∧
+      every_result good_v_i2 good_v_i2 (SND res))``,
+  ho_match_mp_tac evaluate_i3_ind >>
+  strip_tac >- rw[] >>
+  strip_tac >- rw[] >>
+  strip_tac >- rw[] >>
+  strip_tac >- rw[] >>
+  strip_tac >- rw[] >>
+  strip_tac >- rw[] >>
+  strip_tac >- rw[] >>
+  strip_tac >- rw[] >>
+  strip_tac >- (
+    rw[lookup_ALOOKUP,good_env_s_i2_def] >>
+    imp_res_tac ALOOKUP_MEM >>
+    fs[EVERY_MAP,EVERY_MEM,FORALL_PROD] >>
+    metis_tac[] ) >>
+  strip_tac >- rw[] >>
+  strip_tac >- (
+    rw[] >>
+    fs[good_env_s_i2_def,EVERY_MEM,MEM_EL,PULL_EXISTS] >>
+    `n < LENGTH genv` by simp[] >>
+    first_x_assum(qspec_then`n`mp_tac) >>
+    simp[] ) >>
+  strip_tac >- rw[] >>
+  strip_tac >- rw[] >>
+  strip_tac >- ( rw[] >> fs[good_env_s_i2_def] ) >>
+  strip_tac >- (
+    rpt gen_tac >> strip_tac >> strip_tac >> fs[] >>
+    qpat_assum`good_env_s_i2 env s`mp_tac >>
+    qmatch_assum_abbrev_tac`good_env_s_i2 env ss` >>
+    Q.ISPECL_THEN[`env`,`ss`,`uop`,`v`]mp_tac do_uapp_i3_preserves_good  >>
+    simp[Abbr`ss`] ) >>
+  strip_tac >- rw[] >>
+  strip_tac >- rw[] >>
+  strip_tac >- (
+    rpt gen_tac >> strip_tac >> strip_tac >> fs[] >>
+    qspecl_then[`env`,`s3`,`op`,`v1`,`v2`]mp_tac do_app_i2_preserves_good >>
+    simp[] >> fs[good_env_s_i2_def] ) >>
+  strip_tac >- (
+    rw[] >>
+    qspecl_then[`env`,`s3`,`Opapp`,`v1`,`v2`]mp_tac do_app_i2_preserves_good >>
+    simp[] >> fs[good_env_s_i2_def] ) >>
+  strip_tac >- rw[] >>
+  strip_tac >- rw[] >>
+  strip_tac >- rw[] >>
+  strip_tac >- rw[] >>
+  strip_tac >- rw[] >>
+  strip_tac >- rw[] >>
+  strip_tac >- rw[] >>
+  strip_tac >- rw[] >>
+  strip_tac >- ( rw[libTheory.bind_def] >> fs[good_env_s_i2_def] ) >>
+  strip_tac >- rw[] >>
+  strip_tac >- (
+    rpt gen_tac >> strip_tac >> strip_tac >>
+    fs[build_rec_env_i2_MAP,good_env_s_i2_def] >>
+    first_x_assum match_mp_tac >>
+    fs[FST_triple,EVERY_MAP,UNCURRY] >>
+    simp[EVERY_MEM,MEM_MAP,FORALL_PROD,EXISTS_PROD] >>
+    metis_tac[] ) >>
+  strip_tac >- rw[] >>
+  strip_tac >- ( rw[good_env_s_i2_def,EVERY_GENLIST] ) >>
+  strip_tac >- rw[] >>
+  strip_tac >- rw[] >>
+  strip_tac >- rw[] >>
+  strip_tac >- rw[] >>
+  strip_tac >- rw[] >>
+  strip_tac >- ( rw[] >> cheat ) >>
+  strip_tac >- rw[] >>
+  strip_tac >- rw[] >>
+  rw[])
+
+val Let_Els_i4_correct = prove(
+  ``∀n k e tag vs env ck s res us.
+    LENGTH us = n ∧ k ≤ LENGTH vs ∧
+    evaluate_i4 ck (TAKE k vs ++ us ++ (Conv_i4 tag vs::env)) s e res ⇒
+    evaluate_i4 ck (us ++ (Conv_i4 tag vs::env)) s (Let_Els_i4 n k e) res``,
+  ho_match_mp_tac Let_Els_i4_ind >> rw[Let_Els_i4_def] >>
+  rw[Once evaluate_i4_cases] >>
+  disj1_tac >>
+  rw[Once evaluate_i4_cases] >>
+  rw[Once evaluate_i4_cases] >>
+  simp[rich_listTheory.EL_APPEND2] >>
+  simp[do_uapp_i4_def,PULL_EXISTS] >>
+  qmatch_assum_rename_tac`SUC k ≤ LENGTH vs`[] >>
+  first_x_assum(qspecl_then[`tag`,`vs`,`env`,`ck`,`s`,`res`,`EL k vs::us`]mp_tac) >>
+  simp[] >>
+  discharge_hyps >- (
+    fs[arithmeticTheory.ADD1] >>
+    `k < LENGTH vs` by simp[] >>
+    fs[TAKE_EL_SNOC] >>
+    fs[SNOC_APPEND] >>
+    metis_tac[rich_listTheory.CONS_APPEND,APPEND_ASSOC] ) >>
+  PairCases_on`s` >> rw[])
+val Let_Els_i4_correct = prove(
+  ``∀n k e tag vs env ck s res us enve.
+    LENGTH us = n ∧ k ≤ LENGTH vs ∧
+    evaluate_i4 ck (TAKE k vs ++ us ++ (Conv_i4 tag vs::env)) s e res ∧
+    (enve = us ++ (Conv_i4 tag vs::env))
+    ⇒
+    evaluate_i4 ck enve s (Let_Els_i4 n k e) res``,
+  metis_tac[Let_Els_i4_correct])
+
+(* TODO: move *)
+
+(*
+val pat_bindings_i2_acc = store_thm("pat_bindings_i2_acc",
+  ``(∀p l. pat_bindings_i2 p l = pat_bindings_i2 p [] ++ l) ∧
+    (∀ps l. pats_bindings_i2 ps l = pats_bindings_i2 ps [] ++ l)``,
+  ho_match_mp_tac (TypeBase.induction_of``:pat_i2``) >> rw[] >>
+  simp_tac std_ss [pat_bindings_i2_def] >>
+  metis_tac[APPEND,APPEND_ASSOC])
+
+val pmatch_tac =
+  ho_match_mp_tac pmatch_i2_ind >>
+  strip_tac >- (
+    rw[pmatch_i2_def,libTheory.bind_def,pat_bindings_i2_def] >> rw[] ) >>
+  strip_tac >- (
+    rw[pmatch_i2_def,pat_bindings_i2_def] >> rw[] ) >>
+  strip_tac >- ( rw[pmatch_i2_def,pat_bindings_i2_def] ) >>
+  strip_tac >- (
+    rw[pmatch_i2_def,pat_bindings_i2_def] >>
+    Cases_on `store_lookup lnum s`>>
+    fsrw_tac[DNF_ss][semanticPrimitivesTheory.store_lookup_def,EVERY_MEM,MEM_EL]) >>
+  strip_tac >- ( rw[pmatch_i2_def,pat_bindings_i2_def]) >>
+  strip_tac >- rw[pmatch_i2_def] >>
+  strip_tac >- rw[pmatch_i2_def] >>
+  strip_tac >- rw[pmatch_i2_def] >>
+  strip_tac >- rw[pmatch_i2_def] >>
+  strip_tac >- rw[pmatch_i2_def] >>
+  strip_tac >- rw[pmatch_i2_def] >>
+  strip_tac >- ( rw[pmatch_i2_def] >> rw[] ) >>
+  strip_tac >- rw[pmatch_i2_def] >>
+  strip_tac >- rw[pmatch_i2_def] >>
+  strip_tac >- rw[pmatch_i2_def] >>
+  strip_tac >- rw[pmatch_i2_def] >>
+  strip_tac >- (rw[pmatch_i2_def,pat_bindings_i2_def] >> rw[]) >>
+  strip_tac >- (
+    rpt gen_tac >>
+    strip_tac >>
+    simp_tac(srw_ss())[pmatch_i2_def,pat_bindings_i2_def] >>
+    Cases_on `pmatch_i2 s p v env` >> fs[] >>
+    qmatch_assum_rename_tac `pmatch_i2 s p v env = Match env0`[] >>
+    Cases_on `pmatch_list_i2 s ps vs env0` >> fs[] >>
+    simp[Once pat_bindings_i2_acc,SimpRHS]) >>
+  rw[pmatch_i2_def]
+
+val pmatch_i2_dom = store_thm("pmatch_i2_dom",
+  ``(∀s p v env env'.
+      (pmatch_i2 s p v env = Match env') ⇒
+      (MAP FST env' = pat_bindings_i2 p [] ++ (MAP FST env))) ∧
+    (∀s ps vs env env'.
+      (pmatch_list_i2 s ps vs env = Match env') ⇒
+      (MAP FST env' = pats_bindings_i2 ps [] ++ MAP FST env))``,
+    pmatch_tac)
 *)
 
 (*
+val pmatch_list_i2_match_lengths = store_thm("pmatch_list_i2_match_lengths",
+  ``∀ps vs s env env'. pmatch_list_i2 s ps vs env = Match env' ⇒ LENGTH ps = LENGTH vs``,
+  Induct >> TRY(Cases >> simp[pmatch_i2_def] >> NO_TAC) >>
+  gen_tac >> Cases >> simp[pmatch_i2_def] >>
+  rpt gen_tac >> BasicProvers.CASE_TAC >>
+  rw[] >> res_tac)
+*)
+
+val pmatch_list_i2_any = store_thm("pmatch_list_i2_any",
+  ``(∀s p v env env'. pmatch_i2 s p v env = Match env' ⇒
+       ∀env. ∃env'. pmatch_i2 s p v env = Match env') ∧
+    (∀s ps vs env env'. pmatch_list_i2 s ps vs env = Match env' ⇒
+       ∀env. ∃env'. pmatch_list_i2 s ps vs env = Match env')``,
+  ho_match_mp_tac pmatch_i2_ind >>
+  rw[pmatch_i2_def] >>
+  pop_assum mp_tac >>
+  BasicProvers.CASE_TAC >>
+  fs[] >> strip_tac >> fs[] >>
+  BasicProvers.CASE_TAC >> fs[] >>
+  metis_tac[semanticPrimitivesTheory.match_result_distinct])
+
+val pmatch_list_i2_pairwise = store_thm("pmatch_list_i2_pairwise",
+  ``∀ps vs s env env'. pmatch_list_i2 s ps vs env = Match env' ⇒
+      EVERY2 (λp v. ∀env. ∃env'. pmatch_i2 s p v env = Match env') ps vs``,
+  Induct >> Cases_on`vs` >> simp[pmatch_i2_def] >>
+  rpt gen_tac >> BasicProvers.CASE_TAC >> strip_tac >>
+  res_tac >> simp[] >> metis_tac[pmatch_list_i2_any])
+
+val pat_to_i4_Match = prove(
+  ``(∀p v s env env' env4 ck count genv.
+       pmatch_i2 s p v env = Match env' ⇒
+       evaluate_i4 ck
+         (v_to_i4 v::env4)
+         (map_count_store_genv v_to_i4 ((count,s),genv))
+         (pat_to_i4 p)
+         (map_count_store_genv v_to_i4 ((count,s),genv)
+         ,Rval (Litv_i4 (Bool T)))) ∧
+    (∀n ps qs pps vs s env env' env4 ck count genv.
+       pmatch_list_i2 s pps vs env = Match env' ∧
+       (pps = qs ++ ps) ∧ (LENGTH qs = n) ⇒
+       evaluate_i4 ck
+         (vs_to_i4 vs ++ env4)
+         (map_count_store_genv v_to_i4 ((count,s),genv))
+         (pats_to_i4 n ps)
+         (map_count_store_genv v_to_i4 ((count,s),genv)
+         ,Rval (Litv_i4 (Bool T))))``,
+  ho_match_mp_tac pat_to_i4_ind >>
+  rw[pmatch_i2_def,pat_to_i4_def]
+  >- ( rw[Once evaluate_i4_cases] )
+  >- (
+    (Cases_on`v`>>fs[pmatch_i2_def]>>pop_assum mp_tac >> rw[]) >>
+    rw[Once evaluate_i4_cases] >>
+    rw[do_app_i4_def] >>
+    rw[Once evaluate_i4_cases] >>
+    rw[Once evaluate_i4_cases] >>
+    rw[do_eq_i4_def] >>
+    rw[Once evaluate_i4_cases] >>
+    rw[bigStepTheory.dec_count_def,map_count_store_genv_def] )
+  >- (
+    Cases_on`v`>>fs[pmatch_i2_def]>>pop_assum mp_tac >> rw[LENGTH_NIL_SYM] >>
+    rw[Once evaluate_i4_cases] >>
+    rw[do_app_i4_def] >>
+    rw[Once evaluate_i4_cases] >>
+    rw[Once evaluate_i4_cases] >>
+    rw[Once evaluate_i4_cases] >>
+    rw[do_eq_i4_def] >>
+    rw[Once evaluate_i4_cases] >>
+    rw[bigStepTheory.dec_count_def,map_count_store_genv_def] )
+  >- (
+    Cases_on`v`>>fs[pmatch_i2_def]>>pop_assum mp_tac >> rw[] >>
+    rw[Once evaluate_i4_cases] >>
+    rw[Once evaluate_i4_cases] >>
+    rw[Once evaluate_i4_cases] >>
+    rw[do_uapp_i4_def] >>
+    rw[PULL_EXISTS] >>
+    rw[do_if_i4_def] >>
+    fs[map_count_store_genv_def] >>
+    match_mp_tac Let_Els_i4_correct >>
+    simp[LENGTH_NIL,TAKE_LENGTH_ID_rwt] >>
+    first_x_assum match_mp_tac >>
+    simp[LENGTH_NIL] >>
+    metis_tac[])
+  >- (
+    Cases_on`v`>>fs[pmatch_i2_def]>>pop_assum mp_tac >> rw[] >>
+    rw[Once evaluate_i4_cases] >>
+    rw[Once evaluate_i4_cases] >>
+    rw[Once evaluate_i4_cases] >>
+    rw[do_uapp_i4_def,PULL_EXISTS] >>
+    fs[map_count_store_genv_def] >>
+    fs[semanticPrimitivesTheory.store_lookup_def] >>
+    rw[] >> fs[] >> simp[EL_MAP] >>
+    first_x_assum match_mp_tac >>
+    metis_tac[])
+  >- (
+    rw[pat_to_i4_def] >>
+    rw[Once evaluate_i4_cases] ) >>
+  rw[Once evaluate_i4_cases] >>
+  rw[Once evaluate_i4_cases] >>
+  rw[Once evaluate_i4_cases] >>
+  imp_res_tac pmatch_list_i2_pairwise >>
+  `∃ws v rs. (vs = ws ++ v::rs) ∧ LENGTH qs = LENGTH ws` by (
+    qexists_tac`TAKE (LENGTH qs) vs` >>
+    fs[EVERY2_EVERY] >> simp[LENGTH_TAKE] >>
+    qexists_tac`HD (DROP (LENGTH qs) vs)` >>
+    qexists_tac`TL (DROP (LENGTH qs) vs)` >>
+    match_mp_tac EQ_TRANS  >>
+    qexists_tac`TAKE (LENGTH qs) vs ++ DROP (LENGTH qs) vs` >>
+    conj_tac >- metis_tac[TAKE_DROP] >>
+    simp[] >>
+    Cases_on`DROP (LENGTH qs) vs`>>simp[] >>
+    fs[DROP_NIL] >>
+    DECIDE_TAC ) >>
+  rw[] >>
+  simp[rich_listTheory.EL_APPEND2,rich_listTheory.EL_APPEND1] >>
+  qmatch_assum_abbrev_tac`LIST_REL R (l1 ++ l2) (l3 ++ l4)` >>
+  `LIST_REL R l1 l3 ∧ LIST_REL R l2 l4` by (
+    simp[EVERY2_APPEND] >> fs[EVERY2_EVERY] ) >>
+  fs[Abbr`l2`,Abbr`l4`,Abbr`R`] >>
+  first_x_assum(qspec_then`[]`mp_tac) >>
+  disch_then(qx_choose_then`env1`strip_assume_tac) >>
+  first_x_assum(qspecl_then[`v`,`s`,`[]`]mp_tac) >>
+  simp[] >> strip_tac >>
+  qexists_tac`Litv_i4 (Bool T)` >>
+  fs[map_count_store_genv_def] >>
+  simp[do_if_i4_def] >>
+  Q.PAT_ABBREV_TAC`s2 = X:v_i4 count_store_genv` >>
+  qexists_tac`s2` >>
+  conj_tac >- (
+    qunabbrev_tac`s2` >>
+    metis_tac[] ) >>
+  qunabbrev_tac`s2` >>
+  REWRITE_TAC[Once rich_listTheory.CONS_APPEND] >>
+  REWRITE_TAC[APPEND_ASSOC] >>
+  `MAP v_to_i4 l3 ++ [v_to_i4 v] = MAP v_to_i4 (l3 ++ [v])` by simp[] >>
+  pop_assum SUBST1_TAC >>
+  REWRITE_TAC[GSYM MAP_APPEND] >>
+  first_x_assum match_mp_tac >>
+  qexists_tac`l1 ++ [p]` >>
+  qexists_tac`env` >>
+  REWRITE_TAC[GSYM (APPEND_ASSOC)] >>
+  REWRITE_TAC[Once (GSYM rich_listTheory.CONS_APPEND)] >>
+  REWRITE_TAC[GSYM (APPEND_ASSOC)] >>
+  REWRITE_TAC[Once (GSYM rich_listTheory.CONS_APPEND)] >>
+  simp[])
+
+(*
+val drop_def = Define`drop = DROP`
+val pat_to_i4_correct = prove(
+  ``(∀p v s env res env4 ck count genv.
+       pmatch_i2 s p v env = res ∧ res ≠ Match_type_error ⇒
+       evaluate_i4 ck
+         (v_to_i4 v::env4)
+         (map_count_store_genv v_to_i4 ((count,s),genv))
+         (pat_to_i4 p)
+         (map_count_store_genv v_to_i4 ((count,s),genv)
+         ,Rval (Litv_i4 (Bool (∃env'. res = Match env'))))) ∧
+    (∀n ps qs pps vs s env env' res env4 ck count genv.
+       pmatch_list_i2 s (TAKE n pps) (TAKE n vs) env = Match env' ∧
+       pmatch_list_i2 s pps vs env = res ∧ res ≠ Match_type_error ∧
+       (LENGTH ps = LENGTH vs) ∧ n ≤ LENGTH ps ⇒
+       evaluate_i4 ck
+         (vs_to_i4 vs ++ env4)
+         (map_count_store_genv v_to_i4 ((count,s),genv))
+         (pats_to_i4 n ps)
+         (map_count_store_genv v_to_i4 ((count,s),genv)
+         ,Rval (Litv_i4 (Bool (∃env'. res = Match env')))))``,
+  ho_match_mp_tac pat_to_i4_ind >>
+  rw[pmatch_i2_def,pat_to_i4_def]
+  >- ( rw[Once evaluate_i4_cases] )
+  >- (
+    (Cases_on`v`>>fs[pmatch_i2_def]>>pop_assum mp_tac >> rw[]) >>
+    rw[Once evaluate_i4_cases] >>
+    rw[do_app_i4_def] >>
+    rw[Once evaluate_i4_cases] >>
+    rw[Once evaluate_i4_cases] >>
+    rw[do_eq_i4_def] >>
+    rw[Once evaluate_i4_cases] >>
+    rw[bigStepTheory.dec_count_def,map_count_store_genv_def] )
+  >- (
+    Cases_on`v`>>fs[pmatch_i2_def]>>pop_assum mp_tac >> rw[LENGTH_NIL_SYM] >>
+    rw[Once evaluate_i4_cases] >>
+    rw[do_app_i4_def] >>
+    rw[Once evaluate_i4_cases] >>
+    rw[Once evaluate_i4_cases] >>
+    rw[Once evaluate_i4_cases] >>
+    rw[do_eq_i4_def] >>
+    rw[Once evaluate_i4_cases] >>
+    rw[bigStepTheory.dec_count_def,map_count_store_genv_def] >>
+    simp[pmatch_i2_def])
+  >- (
+    Cases_on`v`>>fs[pmatch_i2_def]>>pop_assum mp_tac >> rw[] >>
+    rw[Once evaluate_i4_cases] >>
+    rw[Once evaluate_i4_cases] >>
+    rw[Once evaluate_i4_cases] >>
+    rw[do_uapp_i4_def] >>
+    rw[PULL_EXISTS] >>
+    rw[do_if_i4_def] >>
+    fs[map_count_store_genv_def] >>
+    TRY(simp[Once evaluate_i4_cases] >> NO_TAC) >>
+    match_mp_tac Let_Els_i4_correct >>
+    simp[LENGTH_NIL,TAKE_LENGTH_ID_rwt] >>
+    fs[drop_def])
+  >- (
+    Cases_on`v`>>fs[pmatch_i2_def]>>pop_assum mp_tac >> rw[] >>
+    rw[Once evaluate_i4_cases] >>
+    rw[Once evaluate_i4_cases] >>
+    rw[Once evaluate_i4_cases] >>
+    rw[do_uapp_i4_def,PULL_EXISTS] >>
+    fs[map_count_store_genv_def] >>
+    fs[semanticPrimitivesTheory.store_lookup_def] >>
+    rw[] >> fs[] >> simp[EL_MAP])
+  >- (
+    fs[LENGTH_NIL_SYM,drop_def] >> rw[pmatch_i2_def] >>
+    rw[Once evaluate_i4_cases] )
+  rw[Once evaluate_i4_cases] >>
+  rw[Once evaluate_i4_cases] >>
+  rw[Once evaluate_i4_cases] >>
+  Cases_on`vs`>>fs[]
+  imp_res_tac pmatch_list_i2_pairwise >>
+  `∃ws v rs. (vs = ws ++ v::rs) ∧ LENGTH qs = LENGTH ws` by (
+    qexists_tac`TAKE (LENGTH qs) vs` >>
+    fs[EVERY2_EVERY] >> simp[LENGTH_TAKE] >>
+    qexists_tac`HD (DROP (LENGTH qs) vs)` >>
+    qexists_tac`TL (DROP (LENGTH qs) vs)` >>
+    match_mp_tac EQ_TRANS  >>
+    qexists_tac`TAKE (LENGTH qs) vs ++ DROP (LENGTH qs) vs` >>
+    conj_tac >- metis_tac[TAKE_DROP] >>
+    simp[] >>
+    Cases_on`DROP (LENGTH qs) vs`>>simp[] >>
+    fs[DROP_NIL] >>
+    DECIDE_TAC ) >>
+  rw[] >>
+  simp[rich_listTheory.EL_APPEND2,rich_listTheory.EL_APPEND1] >>
+  qmatch_assum_abbrev_tac`LIST_REL R (l1 ++ l2) (l3 ++ l4)` >>
+  `LIST_REL R l1 l3 ∧ LIST_REL R l2 l4` by (
+    simp[EVERY2_APPEND] >> fs[EVERY2_EVERY] ) >>
+  fs[Abbr`l2`,Abbr`l4`,Abbr`R`] >>
+  first_x_assum(qspec_then`[]`mp_tac) >>
+  disch_then(qx_choose_then`env1`strip_assume_tac) >>
+  first_x_assum(qspecl_then[`v`,`s`,`[]`]mp_tac) >>
+  simp[] >> strip_tac >>
+  qexists_tac`Litv_i4 (Bool T)` >>
+  fs[map_count_store_genv_def] >>
+  simp[do_if_i4_def] >>
+  Q.PAT_ABBREV_TAC`s2 = X:v_i4 count_store_genv` >>
+  qexists_tac`s2` >>
+  conj_tac >- (
+    qunabbrev_tac`s2` >>
+    metis_tac[] ) >>
+  qunabbrev_tac`s2` >>
+  REWRITE_TAC[Once rich_listTheory.CONS_APPEND] >>
+  REWRITE_TAC[APPEND_ASSOC] >>
+  `MAP v_to_i4 l3 ++ [v_to_i4 v] = MAP v_to_i4 (l3 ++ [v])` by simp[] >>
+  pop_assum SUBST1_TAC >>
+  REWRITE_TAC[GSYM MAP_APPEND] >>
+  first_x_assum match_mp_tac >>
+  qexists_tac`l1 ++ [p]` >>
+  qexists_tac`env` >>
+  REWRITE_TAC[GSYM (APPEND_ASSOC)] >>
+  REWRITE_TAC[Once (GSYM rich_listTheory.CONS_APPEND)] >>
+  REWRITE_TAC[GSYM (APPEND_ASSOC)] >>
+  REWRITE_TAC[Once (GSYM rich_listTheory.CONS_APPEND)] >>
+  simp[])
+*)
+
+(*
+val pat_to_i4_No_match = prove(
+  ``(∀p v s env env4 ck count genv.
+       pmatch_i2 s p v env = No_match ⇒
+       evaluate_i4 ck
+         (v_to_i4 v::env4)
+         (map_count_store_genv v_to_i4 ((count,s),genv))
+         (pat_to_i4 p)
+         (map_count_store_genv v_to_i4 ((count,s),genv)
+         ,Rval (Litv_i4 (Bool F)))) ∧
+    (∀n ps vs s env env4 ck count genv.
+       n ≤ LENGTH ps ∧ (LENGTH ps = LENGTH vs) ∧
+       pmatch_list_i2 s (DROP n ps) (DROP n vs) env = No_match ⇒
+       evaluate_i4 ck
+         (vs_to_i4 vs ++ env4)
+         (map_count_store_genv v_to_i4 ((count,s),genv))
+         (pats_to_i4 n ps)
+         (map_count_store_genv v_to_i4 ((count,s),genv)
+         ,Rval (Litv_i4 (Bool F))))``,
+  ho_match_mp_tac pat_to_i4_ind >>
+  rw[pmatch_i2_def,pat_to_i4_def] >- (
+    Cases_on`v`>>fs[pmatch_i2_def]>>
+    pop_assum mp_tac >> rw[] >>
+    rw[Once evaluate_i4_cases] >>
+    rw[Once evaluate_i4_cases] >>
+    rw[Once evaluate_i4_cases] >>
+    rw[do_app_i4_def] >>
+    rw[do_eq_i4_def] >>
+    rw[Once evaluate_i4_cases] >>
+    fs[map_count_store_genv_def] >>
+    rw[bigStepTheory.dec_count_def] )
+  >- (
+    rw[Once evaluate_i4_cases] >>
+    rw[Once evaluate_i4_cases] >>
+    rw[Once evaluate_i4_cases] >>
+    rw[Once evaluate_i4_cases] >>
+    rw[do_app_i4_def] >>
+    Cases_on`v`>>fs[pmatch_i2_def]>>
+    pop_assum mp_tac >> rw[LENGTH_NIL_SYM,pmatch_i2_def] >>
+    rw[do_eq_i4_def] >>
+    rw[Once evaluate_i4_cases] >>
+    fs[map_count_store_genv_def] >>
+    rw[bigStepTheory.dec_count_def] )
+  >- (
+    rw[Once evaluate_i4_cases] >>
+    rw[Once evaluate_i4_cases] >>
+    rw[Once evaluate_i4_cases] >>
+    rw[do_uapp_i4_def] >>
+    Cases_on`v`>>fs[pmatch_i2_def]>>
+    pop_assum mp_tac >> rw[] >- (
+      fs[LENGTH_NIL] >>
+      simp[PULL_EXISTS] >>
+      simp[do_if_i4_def] >>
+      fs[map_count_store_genv_def] >>
+      match_mp_tac Let_Els_i4_correct >>
+      simp[LENGTH_NIL] >>
+      simp[TAKE_LENGTH_ID_rwt] >>
+      first_x_assum match_mp_tac >>
+      metis_tac[] ) >>
+    simp[PULL_EXISTS] >>
+    simp[do_if_i4_def] >>
+    simp[Once evaluate_i4_cases] >>
+    simp[map_count_store_genv_def] )
+  >- (
+    rw[Once evaluate_i4_cases] >>
+    rw[Once evaluate_i4_cases] >>
+    rw[Once evaluate_i4_cases] >>
+    rw[do_uapp_i4_def] >>
+    Cases_on`v`>>fs[pmatch_i2_def]>>
+    simp[PULL_EXISTS] >>
+    fs[map_count_store_genv_def] >>
+    fs[semanticPrimitivesTheory.store_lookup_def] >>
+    rw[] >> fs[] >>
+    simp[EL_MAP] >>
+    first_x_assum match_mp_tac >>
+    metis_tac[] )
+  >- (
+    fs[LENGTH_NIL_SYM] >>
+    rfs[pmatch_i2_def] )
+  >- (
+    Cases_on`vs`>>fs[] >>
+    rw[Once evaluate_i4_cases] >>
+    rw[Once evaluate_i4_cases] >>
+    rw[Once evaluate_i4_cases] >>
+    fs[pmatch_i2_def] >>
+    pop_assum mp_tac >> BasicProvers.CASE_TAC >- (
+      qexists_tac`Litv_i4 (Bool F)` >>
+      simp[do_if_i4_def] >>
+      metis_tac[CONJUNCT1 evaluate_i4_rules] ) >>
+    rw[] >>
+    qexists_tac`Litv_i4 (Bool T)` >>
+    rw[do_if_i4_def] >>
+    imp_res_tac(CONJUNCT1 pat_to_i4_Match)
+
+
+      res_tac >> pop_assum mp_tac >>
+      simp[Once evaluate_i4_cases] >>
+      simp[Once evaluate_i4_cases] >>
+*)
+
 val exp_to_i4_correct = store_thm("exp_to_i4_correct",
   ``(∀ck env s exp res. evaluate_i3 ck env s exp res ⇒
-     (SND res ≠ Rerr Rtype_error) ∧ every_result good_v_i2 good_v_i2 (SND res) ⇒
+     (SND res ≠ Rerr Rtype_error) ∧ good_env_s_i2 env s ⇒
      evaluate_i4 ck
        (MAP (v_to_i4 o SND) env)
        (map_count_store_genv v_to_i4 s)
@@ -243,7 +795,7 @@ val exp_to_i4_correct = store_thm("exp_to_i4_correct",
        (map_count_store_genv v_to_i4 (FST res)
        ,map_result v_to_i4 v_to_i4 (SND res))) ∧
     (∀ck env s exps ress. evaluate_list_i3 ck env s exps ress ⇒
-     (SND ress ≠ Rerr Rtype_error) ∧ every_result good_vs_i2 good_v_i2 (SND ress) ⇒
+     (SND ress ≠ Rerr Rtype_error) ∧ good_env_s_i2 env s ⇒
      evaluate_list_i4 ck
        (MAP (v_to_i4 o SND) env)
        (map_count_store_genv v_to_i4 s)
@@ -251,20 +803,20 @@ val exp_to_i4_correct = store_thm("exp_to_i4_correct",
        (map_count_store_genv v_to_i4 (FST ress)
        ,map_result vs_to_i4 v_to_i4 (SND ress))) ∧
     (∀ck env s v pes ev res. evaluate_match_i3 ck env s v pes ev res ⇒
-      (SND res ≠ Rerr Rtype_error) ∧ every_result good_v_i2 good_v_i2 (SND res) ⇒
+      (SND res ≠ Rerr Rtype_error) ∧ good_env_s_i2 env s ⇒
       evaluate_i4 ck
       (v_to_i4 v::(MAP (v_to_i4 o SND) env))
       (map_count_store_genv v_to_i4 s)
       (pes_to_i4 (NONE::(MAP (SOME o FST) env)) pes)
       (map_count_store_genv v_to_i4 (FST res)
       ,map_result v_to_i4 v_to_i4 (SND res)))``
-  ho_match_mp_tac evaluate_i3_ind >>
+  ho_match_mp_tac evaluate_i3_strongind >>
   strip_tac >- rw[Once evaluate_i4_cases] >>
   strip_tac >- ( rw[] >> simp[Once evaluate_i4_cases] ) >>
   strip_tac >- ( rw[] >> simp[Once evaluate_i4_cases] ) >>
   strip_tac >- ( rw[] >> simp[Once evaluate_i4_cases] ) >>
   strip_tac >- (
-    rw[] >> simp[Once evaluate_i4_cases] >> metis_tac[] ) >>
+    rw[] >> simp[Once evaluate_i4_cases] >> metis_tac[evaluate_i3_preserves_good,FST] ) >>
   strip_tac >- ( rw[] >> simp[Once evaluate_i4_cases] ) >>
   strip_tac >- ( rw[] >> simp[Once evaluate_i4_cases] ) >>
   strip_tac >- ( rw[] >> simp[Once evaluate_i4_cases] ) >>
@@ -287,6 +839,7 @@ val exp_to_i4_correct = store_thm("exp_to_i4_correct",
     Cases_on`uop`>>
     fs[do_uapp_i3_def,do_uapp_i4_def,LET_THM,semanticPrimitivesTheory.store_alloc_def] >>
     rw[] >>
+    pop_assum kall_tac >>
     TRY (pop_assum mp_tac >> BasicProvers.CASE_TAC) >>
     simp[semanticPrimitivesTheory.store_lookup_def] >> rw[] >>
     fs[map_count_store_genv_def] >>
@@ -301,18 +854,124 @@ val exp_to_i4_correct = store_thm("exp_to_i4_correct",
     rpt gen_tac >> strip_tac >> strip_tac >> fs[] >>
     simp[Once evaluate_i4_cases] >> disj1_tac >>
     map_every qexists_tac[`v_to_i4 v1`,`v_to_i4 v2`] >>
-    qmatch_assum_abbrev_tac`evaluate_i4 A B C D E` >>
+    qmatch_assum_abbrev_tac`P ⇒ evaluate_i4 A B C D E` >>
     map_every qexists_tac[`B`,`D`] >>
     qmatch_assum_abbrev_tac`evaluate_i4 a b c d (e,Rval (v_to_i4 v1))` >>
     qexists_tac`e` >> unabbrev_all_tac >>
     fs[map_count_store_genv_def] >>
-    qmatch_assum_abbrev_tac`evaluate_i4 a b c d (((e,f),g),Rval (v_to_i4 v2))` >>
-    map_every qexists_tac[`f`,`e`] >>
-    qmatch_assum_abbrev_tac`evaluate_i4 A B ((C,D),E) G H` >>
+    qmatch_assum_abbrev_tac`p ⇒ evaluate_i4 a b c d (((e,f),g),Rval (v_to_i4 v2))` >>
+    `p` by metis_tac[evaluate_i3_preserves_good,FST] >>
+    map_every qexists_tac[`f`,`e`] >> qunabbrev_tac`p` >> fs[] >>
+    qmatch_assum_abbrev_tac`q ⇒ evaluate_i4 A B ((C,D),E) G H` >>
+    `good_v_i2 v1 ∧ q` by (
+      unabbrev_all_tac >>
+      imp_res_tac evaluate_i3_preserves_good >>
+      imp_res_tac do_app_i2_preserves_good >>
+      rfs[good_env_s_i2_def] ) >>
+    fs[Abbr`q`] >>
     map_every qexists_tac[`D`,`E`] >> unabbrev_all_tac >>
     simp[] >>
-    qpat_assum`do_app_i2 A B C D E = G`mp_tac >>
-*)
+    simp[do_app_i4_correct] ) >>
+  strip_tac >- (
+    rw[] >> simp[Once evaluate_i4_cases] >>
+    imp_res_tac evaluate_i3_preserves_good >>
+    rfs[] >> fs[] >>
+    qspecl_then[`Opapp`,`v1`,`v2`,`env`,`s3`]mp_tac do_app_i4_correct >>
+    simp[] >> fs[map_count_store_genv_def] >> metis_tac[] ) >>
+  strip_tac >- rw[] >>
+  strip_tac >- (
+    rw[] >> simp[Once evaluate_i4_cases] >>
+    imp_res_tac evaluate_i3_preserves_good >>
+    fs[] >> metis_tac[] ) >>
+  strip_tac >- (
+    rw[] >> simp[Once evaluate_i4_cases] ) >>
+  strip_tac >- (
+    rw[] >> simp[Once evaluate_i4_cases] >>
+    imp_res_tac evaluate_i3_preserves_good >>
+    fs[do_if_i2_def,do_if_i4_def] >>
+    disj1_tac >>
+    qexists_tac`v_to_i4 v` >>
+    Cases_on`v`>>fs[]>>
+    Cases_on`l`>>fs[]>>
+    Cases_on`b`>>fs[]>>
+    metis_tac[]) >>
+  strip_tac >- rw[] >>
+  strip_tac >- (
+    rw[] >> simp[Once evaluate_i4_cases] ) >>
+  strip_tac >- (
+    rw[] >> simp[Once evaluate_i4_cases] >>
+    metis_tac[evaluate_i3_preserves_good,FST] ) >>
+  strip_tac >- (
+    rw[] >> simp[Once evaluate_i4_cases] ) >>
+  strip_tac >- (
+    rw[] >> simp[Once evaluate_i4_cases] >>
+    fs[libTheory.bind_def] >>
+    disj1_tac >>
+    imp_res_tac evaluate_i3_preserves_good >>
+    fs[good_env_s_i2_def] >> metis_tac[] ) >>
+  strip_tac >- (
+    rw[] >> simp[Once evaluate_i4_cases] ) >>
+  strip_tac >- (
+    rw[] >> simp[Once evaluate_i4_cases] >>
+    `good_env_s_i2 (build_rec_env_i2 funs env env) s` by (
+      simp[build_rec_env_i2_MAP] >>
+      fs[good_env_s_i2_def,EVERY_MAP,EVERY_MEM,FST_triple,UNCURRY] >>
+      simp[MEM_MAP] >> metis_tac[] ) >>
+    fs[] >>
+    qmatch_abbrev_tac`evaluate_i4 a b c d e` >>
+    qmatch_assum_abbrev_tac`evaluate_i4 a b' c d' e` >>
+    `b = b'` by (
+      unabbrev_all_tac >>
+      fs[build_rec_env_i4_def,build_rec_env_i2_MAP,funs_to_i4_MAP] >>
+      rw[LIST_EQ_REWRITE,EL_MAP,UNCURRY,funs_to_i4_MAP] >- (
+        rpt (AP_THM_TAC ORELSE AP_TERM_TAC) >>
+        simp[FUN_EQ_THM,FORALL_PROD] ) >>
+      fs[FST_triple] >>
+      imp_res_tac find_index_ALL_DISTINCT_EL >>
+      first_x_assum(qspec_then`x`mp_tac) >>
+      discharge_hyps >- simp[] >>
+      disch_then(qspec_then`0`mp_tac) >>
+      asm_simp_tac(std_ss)[EL_MAP] >>
+      simp[]) >>
+    `d = d'` by (
+      unabbrev_all_tac >>
+      simp[build_rec_env_i2_MAP] >>
+      rpt (AP_THM_TAC ORELSE AP_TERM_TAC) >>
+      simp[MAP_MAP_o,combinTheory.o_DEF] >>
+      rpt (AP_THM_TAC ORELSE AP_TERM_TAC) >>
+      simp[FUN_EQ_THM,FORALL_PROD] ) >>
+    rw[] ) >>
+  strip_tac >- rw[] >>
+  strip_tac >- (
+    rw[] >>
+    simp[Once evaluate_i4_cases] >>
+    simp[map_count_store_genv_def,MAP_GENLIST,combinTheory.o_DEF] ) >>
+  strip_tac >- ( rw[] >> simp[Once evaluate_i4_cases] ) >>
+  strip_tac >- (
+    rw[] >> simp[Once evaluate_i4_cases] >>
+    metis_tac[evaluate_i3_preserves_good,FST] ) >>
+  strip_tac >- (
+    rw[] >> simp[Once evaluate_i4_cases] ) >>
+  strip_tac >- (
+    rw[] >> simp[Once evaluate_i4_cases] >>
+    metis_tac[evaluate_i3_preserves_good,FST] ) >>
+  strip_tac >- (
+    rw[] >> simp[Once evaluate_i4_cases] >>
+    cheat (* false - want i3 pattern matches to be exhaustive but they aren't *) ) >>
+  strip_tac >- (
+    rw[] >>
+    simp[Once evaluate_i4_cases] >>
+    disj1_tac >>
+    qexists_tac`Litv_i4 (Bool T)` >>
+    simp[do_if_i4_def] >>
+    imp_res_tac(CONJUNCT1 pat_to_i4_Match) >>
+    Q.PAT_ABBREV_TAC`s2 = X:v_i4 count_store_genv` >>
+    qexists_tac`s2` >> simp[Abbr`s2`] >>
+    cheat ) >>
+  strip_tac >- (
+    rw[] >> cheat ) >>
+  strip_tac >- rw[] >>
+  rw[])
 
 
 (*
